Change to try prove simpler calculus

CPL/c_tableau_calculus.v
@@ -8,12 +8,13 @@ Definition Tableau : Type := list PropF.
 
 Inductive ClosedT_P : Tableau -> Prop :=
   | TId    : forall L A       , In A L -> In (¬A) L                  -> ClosedT_P L
-  | TAnd   : forall L1 L2 A B , ClosedT_P (L1++A::B::L2) -> ClosedT_P (L1++A∧B::L2)
-  | TOr    : forall L1 L2 A B , ClosedT_P (L1++A::L2) -> ClosedT_P (L1++B::L2) -> ClosedT_P (L1++A∨B::L2)
+  | TAnd  : forall L1 L2 A B , ClosedT_P (L1++A::B::L2) -> ClosedT_P (L1++A∧B::L2)
+  | TNAnd  : forall L1 L2 A B , ClosedT_P (L1++¬A::L2) -> ClosedT_P (L1++¬B::L2) -> ClosedT_P (L1++¬(A∧B)::L2)
+  (*| TOr    : forall L1 L2 A B , ClosedT_P (L1++A::L2) -> ClosedT_P (L1++B::L2) -> ClosedT_P (L1++A∨B::L2)
   | TImp   : forall L1 L2 A B , ClosedT_P (L1++¬A::L2) -> ClosedT_P (L1++B::L2) -> ClosedT_P (L1++A→B::L2)
   | TNAnd  : forall L1 L2 A B , ClosedT_P (L1++¬A::L2) -> ClosedT_P (L1++¬B::L2) -> ClosedT_P (L1++¬(A∧B)::L2)
   | TNOr   : forall L1 L2 A B , ClosedT_P (L1++¬A::¬B::L2) -> ClosedT_P (L1++¬(A∨B)::L2)
   | TNImp  : forall L1 L2 A B , ClosedT_P (L1++A::¬B::L2) -> ClosedT_P (L1++¬(A→B)::L2)
-.
+*).
 
 End tableau_calculus_mod.
