CPL/b_sequent_calculus.v
@@ -12,13 +12,16 @@ Notation "Γ ⇒ Δ" := (Arrow Γ Δ) (at level 80): My_scope.
 
 Inductive DerSeq_P : Seq -> Prop :=
   | SId   : forall A Γ Δ      , In A Γ                      -> In A Δ                     -> DerSeq_P (Γ ⇒ Δ)
-  | SBotL : forall Γ Δ        , In ⊥ Γ                                                    -> DerSeq_P (Γ ⇒ Δ)
+  | SBotL : forall A Γ1 Γ2 Δ1 Δ2  , DerSeq_P (Γ1++Γ2 ⇒ Δ1++A::Δ2) -> DerSeq_P (Γ1++¬A::Γ2 ⇒ Δ1++Δ2)
+  | SBotR : forall A Γ1 Γ2 Δ1 Δ2  , DerSeq_P (Γ1++A::Γ2 ⇒ Δ1++Δ2) -> DerSeq_P (Γ1++Γ2 ⇒ Δ1++¬A::Δ2)
+  | SRBotL : forall A Γ1 Γ2 Δ1 Δ2  , DerSeq_P (Γ1++¬A::Γ2 ⇒ Δ1++Δ2) -> DerSeq_P (Γ1++Γ2 ⇒ Δ1++A::Δ2)
+  | SRBotR : forall A Γ1 Γ2 Δ1 Δ2  , DerSeq_P (Γ1++Γ2 ⇒ Δ1++¬A::Δ2) -> DerSeq_P (Γ1++A::Γ2 ⇒ Δ1++Δ2)
   | SAndL : forall A B Γ1 Γ2 Δ, DerSeq_P (Γ1++A::B::Γ2 ⇒ Δ)                               -> DerSeq_P (Γ1++A∧B::Γ2 ⇒ Δ)
   | SAndR : forall A B Γ Δ1 Δ2, DerSeq_P (Γ ⇒ Δ1++A::Δ2)    -> DerSeq_P (Γ ⇒ Δ1++B::Δ2)   -> DerSeq_P (Γ ⇒ Δ1++A∧B::Δ2)
-  | SOrL  : forall A B Γ1 Γ2 Δ, DerSeq_P (Γ1++A::Γ2 ⇒ Δ)    -> DerSeq_P (Γ1++B::Γ2 ⇒ Δ)   -> DerSeq_P (Γ1++A∨B::Γ2 ⇒ Δ)
+  (*| SOrL  : forall A B Γ1 Γ2 Δ, DerSeq_P (Γ1++A::Γ2 ⇒ Δ)    -> DerSeq_P (Γ1++B::Γ2 ⇒ Δ)   -> DerSeq_P (Γ1++A∨B::Γ2 ⇒ Δ)
   | SOrR  : forall A B Γ Δ1 Δ2, DerSeq_P (Γ ⇒ Δ1++A::B::Δ2)                               -> DerSeq_P (Γ ⇒ Δ1++A∨B::Δ2)
   | SImpL : forall A B Γ1 Γ2 Δ, DerSeq_P (Γ1++B::Γ2 ⇒ Δ)    -> DerSeq_P (Γ1++Γ2 ⇒ A::Δ)   -> DerSeq_P (Γ1++A→B::Γ2 ⇒ Δ)
   | SImpR : forall Γ Δ1 Δ2 A B, DerSeq_P (A::Γ ⇒ Δ1++B::Δ2)                               -> DerSeq_P (Γ ⇒ Δ1++A→B::Δ2)
-.
+*).
 
 End sequent_calculus_mod.
